\documentclass[12pt,a4paper,draft]{article}
\usepackage[utf8]{inputenc}
\usepackage{amsmath}
\usepackage{amsfonts}
\usepackage{amssymb}
\usepackage{graphicx}
\usepackage{bm}


\begin{document}
The log likelihood:
\begin{align*}
	l(\bm{\beta},\bm{N}; \bm{t}) &=
	\sum_{t_i \in \bm t} \sum_{j=1}^\infty \left[
		I\{ x_{t_i} = j \} \log(\lambda_{j,t_i}) -
		\lambda_{j,t_i} \Delta_i
	\right]	
\end{align*}

where 
\begin{align*}
	\lambda_{j,t_i} &:= \beta_j I_{t_i} (N_j-n_{j,t_i}) \\
	\Delta_i &:= t_i - t_{i-1}. 
\end{align*}

By differentiating w.r.t. $N_k$:
\begin{align}\label{eq:Nk_FOC}
\begin{split}
	\sum_{t_i:x_{t_i}=k} \frac{1}{N_k - n_{k,t_i}} &= A_k \beta_k \\
	A_k &:= \sum_{t_i \in \bm t} I_{t_i} \Delta_i
\end{split}
\end{align}

By differentiating w.r.t. $\beta_k$
\begin{align}\label{eq:beta_FOC}
\begin{split}
	n_k &= \beta_k [ N_k A_k- B ] \\
	n_k &:= \sum_{t_i:x_{t_i}=k} 1 \\
	B_k &:= \sum_{t_i \in \bm t} I_{t_i} \, n_{k,t_i} \, \Delta_i.
\end{split}
\end{align}

Solving for $\beta_k$ and plugging in Eq.\ref{eq:Nk_FOC}
\begin{align}\label{eq:partial_likelihood}
\begin{split}
	\left( N_k-\frac{B_k}{A_k} \right) 
	\left( \sum_{t_i:x_{t_i}=k}\frac{1}{N_k - n_{k,t_i}}\right) - n_{k}=0
\end{split}
\end{align}

It thus remains to find the root(s) of Eq.\ref{eq:partial_likelihood} to find $\hat{N}_k$ and plug it in Eq~\ref{eq:beta_FOC} to find $\hat{\beta}_k$.

\hrulefill
\bigskip

Now adding some regularization via Jefrey's prior...





\end{document}